wip generalizing monad-related tc instances

src/Lean4Lean/Ext.lean
@@ -7,7 +7,6 @@ def toKernelException (m : EIO Exception α) : EIO KernelException (Sum α Excep
   | .ok s I => .ok (.inl s) I
   | .error e I => .ok (.inr e) I
 
-
 def runMetaM (m : MetaM T) : RecM T := do
   let mut options := (← readThe Context).options
   let m' := Lean.Meta.MetaM.run m {lctx := (← readThe Context).lctx, fuel := (← readThe Context).fuel - 1} |>.run {options := options, fileName := default, fileMap := default, maxHeartbeats := 0} {env := (← readThe Context).env'}
@@ -16,6 +15,62 @@ def runMetaM (m : MetaM T) : RecM T := do
   | .inr (.internal _ _) => throw $ .other "untranslated Exception.Internal"
   | .inr (.error _ d) => throw $ .other (← d.toString)
 
+def apply (mvarId : MVarId) (e : Expr) (eType? : Option Expr := none) : RecMO T (List MVarId) :=
+  mvarId.withContext do
+    mvarId.checkNotAssigned `apply
+    let targetType ← mvarId.getType
+    let eType      ← eType?.getDM (inferType e)
+    let (numArgs, hasMVarHead) ← getExpectedNumArgsAux eType
+    /-
+    The `apply` tactic adds `_`s to `e`, and some of these `_`s become new goals.
+    When `hasMVarHead` is `false` we try different numbers, until we find a type compatible with `targetType`.
+    We used to try only `numArgs-targetTypeNumArgs` when `hasMVarHead = false`, but this is not always correct.
+    For example, consider the following example
+    ```
+    example {α β} [LE_trans β] (x y z : α → β) (h₀ : x ≤ y) (h₁ : y ≤ z) : x ≤ z := by
+      apply le_trans
+      assumption
+      assumption
+    ```
+    In this example, `targetTypeNumArgs = 1` because `LE` for functions is defined as
+    ```
+    instance {α : Type u} {β : Type v} [LE β] : LE (α → β) where
+      le f g := ∀ i, f i ≤ g i
+    ```
+    -/
+    let rangeNumArgs ← if hasMVarHead then
+      pure [numArgs : numArgs+1]
+    else
+      let targetTypeNumArgs ← getExpectedNumArgs targetType
+      pure [numArgs - targetTypeNumArgs : numArgs+1]
+    /-
+    Auxiliary function for trying to add `n` underscores where `n ∈ [i: rangeNumArgs.stop)`
+    See comment above
+    -/
+    let rec go (i : Nat) : MetaM (Array Expr × Array BinderInfo) := do
+      if i < rangeNumArgs.stop then
+        let s ← saveState
+        let (newMVars, binderInfos, eType) ← forallMetaTelescopeReducing eType i
+        if (← isDefEqApply cfg eType targetType) then
+          return (newMVars, binderInfos)
+        else
+          s.restore
+          go (i+1)
+      else
+        let (_, _, eType) ← forallMetaTelescopeReducing eType (some rangeNumArgs.start)
+        throwApplyError mvarId eType targetType
+      termination_by rangeNumArgs.stop - i
+    let (newMVars, binderInfos) ← go rangeNumArgs.start
+    postprocessAppMVars `apply mvarId newMVars binderInfos cfg.synthAssignedInstances cfg.allowSynthFailures
+    let e ← instantiateMVars e
+    mvarId.assign (mkAppN e newMVars)
+    let newMVars ← newMVars.filterM fun mvar => not <$> mvar.mvarId!.isAssigned
+    let otherMVarIds ← getMVarsNoDelayed e
+    let newMVarIds ← reorderGoals newMVars cfg.newGoals
+    let otherMVarIds := otherMVarIds.filter fun mvarId => !newMVarIds.contains mvarId
+    let result := newMVarIds ++ otherMVarIds.toList
+    result.forM (·.headBetaType)
+    return result
 
 open Lean.Meta in
 def extMatch (getT : MetaM (Expr × List Expr)) (localMarker : Name) (lems : List Name) (dbg := false) : RecMO T (Option (Expr × List Expr)) := do
@@ -26,33 +81,32 @@ def extMatch (getT : MetaM (Expr × List Expr)) (localMarker : Name) (lems : Lis
   -- if dbg then 
   --   dbg_trace s!"DBG[387]: TypeChecker.lean:406 (after if dbg then)"
 
-  let ret? ← runMetaM (do
+  let ret? ← (do
     let mut localLems := []
     for decl in (← getLCtx) do
       if dbg then 
         dbg_trace s!"Checking: {decl.userName} : {← ppExpr decl.type}"
       if let .app (.const n []) _ := decl.type.getForallBody then -- TODO remove once we can generate lemmas for intermediate reducts
         if n == localMarker then
-          let newType ← forallTelescope decl.type fun vs b => mkForallFVars vs b.appArg!
+          let newType ← liftM $ forallTelescope decl.type fun vs b => mkForallFVars vs b.appArg!
           localLems := localLems ++ [(decl.toExpr, .some newType)]
           if dbg then 
             dbg_trace s!"Added: {decl.userName} : {← ppExpr decl.type}"
 
     let mut candidates := (← lems.mapM (mkConstWithFreshMVarLevels ·)).zip (List.replicate lems.length none)
     candidates := candidates ++ localLems
-    withLCtx' (← read).lctx do
-      let (T, _) ← getT
-      let condString := do pure s!"{← ppExpr $ ← T.mvarId!.getType}"
-      -- let dbg := (← readThe Core.Context).options.get? `trace.Kernel.ext
-      trace[Kernel.ext] "Trying to show {← condString}"
-      let tryExtEq lem type? T ts := do
+    liftM $ withLCtx' (← read).lctx do
+      let tryExtEq lem type? (T : Expr) (ts : List Expr) := do
+        let condString := do pure s!"{← ppExpr $ ← T.mvarId!.getType}"
+        -- let dbg := (← readThe Core.Context).options.get? `trace.Kernel.ext
+        trace[Kernel.ext] "Trying to show {← condString}"
         try
           trace[Kernel.ext] s!"Trying to apply (fuel {(← read).fuel}): {← ppExpr $ lem} : {← ppExpr $ (← Meta.inferType lem)} to {← condString}"
           let gs ← T.mvarId!.apply lem (cfg := {shallow := true}) type?
 
-          trace[Kernel.ext] s!"Applying OK:{← ppExpr $ (← Meta.inferType lem)} to  {← condString}\n  {← gs.mapM (do ppExpr $ ← ·.getType)}\n  {← localLems.mapM (do ppExpr $ ← Meta.inferType ·.1)}"
+          trace[Kernel.ext] s!"Applying OK:{← ppExpr $ (← Meta.inferType lem)} to  {← condString}" --"\n  {← gs.mapM (fun (id : MVarId) => do ppExpr $ ← id.getType)}\n  {← localLems.mapM (do ppExpr $ ← Meta.inferType ·.1)}"
           if dbg then
-            dbg_trace s!"Applying OK:{← ppExpr $ (← Meta.inferType lem)} to  {← condString}\n  {← gs.mapM (do ppExpr $ ← ·.getType)}\n  {← localLems.mapM (do ppExpr $ ← Meta.inferType ·.1)}"
+            dbg_trace s!"Applying OK:{← ppExpr $ (← Meta.inferType lem)} to  {← condString}" --"\n  {← gs.mapM (do ppExpr $ ← ·.getType)}\n  {← localLems.mapM (do ppExpr $ ← Meta.inferType ·.1)}"
           for g in gs do
             -- TODO unassign T if any g.refl fails?
             try
@@ -71,11 +125,12 @@ def extMatch (getT : MetaM (Expr × List Expr)) (localMarker : Name) (lems : Lis
           if dbg then
             dbg_trace s!"Applying FAIL: {← ppExpr $ lem} : {← ppExpr $ (← Meta.inferType lem)} to {← condString}"
           pure none
+      let (T, ts) ← getT
+
       for (lem, type?) in candidates do
         -- for eqMvar in [tEqsMvar, sEqtMvar] do
         -- TODO is there a way to "undo" assignments from previous failed unification attempts,
         -- rather than making new mvars every time?
-        let (T, ts) ← getT
         if let .some prf ← tryExtEq lem type? T ts then
           printTraces
           return some prf
@@ -86,7 +141,7 @@ def extMatch (getT : MetaM (Expr × List Expr)) (localMarker : Name) (lems : Lis
 
   if let some (prf, ts) := ret? then
     if prf.hasExprMVar then
-      throw $ .other "unexpected mvar found in extensional equality proof"
+      Lean.throwError "unexpected mvar found in extensional equality proof"
     if ts.any (·.hasExprMVar) then
       throw $ .other "unexpected mvar found in extensionally assigned variable"
     -- check that the proof returned by unification is well-typed with the kernel itself,
