src/Lean4Lean/RecM.lean
@@ -36,11 +36,21 @@ structure TypeChecker.Context where
 
 namespace TypeChecker
 
-abbrev M := ReaderT Context <| StateT State <| EIO KernelException
+instance (ω σ : Type) : MonadControl MetaM (StateT ω MetaM) :=
+  inferInstance
+
+instance (ω σ : Type) : MonadControl MetaM (StateT ω MetaM) :=
+  inferInstance
+
+abbrev M := ReaderT Context <| StateT State <| MetaM
+
+instance : MonadControlT MetaM (M) :=
+  inferInstance
+
 abbrev MO (T : Type) := ContT T M
 
 def M.run (env : Kernel.Environment) (env' : Environment) (safety : DefinitionSafety := .safe) (lctx : LocalContext := {}) (options : Options)
-    (x : M α) (fuel := 5) (localDfEqs : List Expr := []) : EIO KernelException α :=
+    (x : M α) (fuel := 5) (localDfEqs : List Expr := []) : MetaM α :=
   x { env, env', safety, lctx, fuel, options } |>.run' {}
 
 -- instance : MonadEnv M where
@@ -94,3 +104,13 @@ def whnfCore (e : Expr) (l : Option (Level × Expr) := none) (cheapRec := false)
 def whnf (e : Expr) (d : Option (Level × Expr) := none) : RecMO T Expr := fun f m => m.whnf e d fun e => f e m
 
 def inferType (e : Expr) (inferOnly := true) : RecMO T Expr := fun f m => m.inferType e inferOnly fun a => f a m
+
+set_option trace.Meta.synthInstance true in
+instance : MonadQuotation RecM :=
+  inferInstance
+#print instMonadQuotationOfMonadFunctorOfMonadLift
+instance : MonadError Lean.Elab.Tactic.TacticM :=
+  inferInstance
+set_option pp.explicit true in
+-- #print instAddErrorMessageContextOfAddMessageContextOfMonad
+#print Lean.TypeChecker.Inner.instMonadErrorTacticM_lean4Lean
